\documentclass[11pt,a4paper]{jsarticle}

\usepackage{amsmath,amssymb}

\newcommand{\E}{\mathrm{E}}

\begin{document}

例18

\begin{align}
F_n (1, \theta)
& =
- \log \int_0^1 dx \int_0^1 dy \, \exp ( -n x^2 y^\theta ) \nonumber
\end{align}

$K(x, y) = x^2 y^\theta$とおく．
\begin{align}
F_n (1, \theta)
& =
- \log \int_{-\infty}^{\infty} dt \int_0^1 dx \int_0^1 dy \, \exp(-t) \delta \bigl( t - n K(x, y) \bigr) \nonumber \\
& =
- \log \int_0^n \frac{dt}{n} \int_0^1 dx \int_0^1 dy \, \exp(-t) \delta \Bigl( \frac{t}{n} - K(x, y) \Bigr) \nonumber
\end{align}

$2k = (2, \theta), \, h = (0, 0)$より，$\lambda = \min \bigl\{ 1/2, 1/\theta \bigr\}$．

$\theta < 2$のとき．
$\lambda = 1/2, \, m = 1$より
\begin{align}
\frac{1}{(m - 1)! 2^m \prod_{j=1}^m k_j}
& =
\frac{1}{2}, \nonumber \\
\mu_2
& =
-\frac{\theta}{2} \nonumber \\
\delta \bigl( t - K(x, y) \bigr)
& \simeq
\frac{1}{2} t^{-1/2} \delta(x) y^{-\theta/2} \nonumber
\end{align}

$\theta = 2$のとき．
$\lambda = 1/2, \, m = 2$より
\begin{align}
\frac{1}{(m - 1)! 2^m \prod_{j=1}^m k_j}
& =
\frac{1}{4}, \nonumber \\
\delta \bigl( t - K(x, y) \bigr)
& \simeq
\frac{1}{4} t^{-1/2} (-\log t) \delta(x) \delta(y) \nonumber
\end{align}

$\theta > 2$のとき．
$\lambda = 1/\theta, \, m = 1$より
\begin{align}
\frac{1}{(m - 1)! 2^m \prod_{j=1}^m k_j}
& =
\frac{1}{\theta}, \nonumber \\
\mu_2
& =
-\frac{2}{\theta} \nonumber \\
\delta \bigl( t - K(x, y) \bigr)
& \simeq
\frac{1}{\theta} t^{1/\theta - 1} x^{-2/\theta} \delta(y) \nonumber
\end{align}

例19

\begin{align}
F_n (1, \theta)
& =
- \log \int_0^1 dx \int_{\| y \| < 1} dy \, \exp ( -n x^2 \| y \|^2 ) x^{\theta - 1} \nonumber \\
& =
- \log \int_0^1 dx \int_0^1 dr \int d \psi \, \exp ( -n x^2 r^2 ) x^{\theta - 1} r^{M - 1} \nonumber
\end{align}

$K(x, r) = x^2 r^2$とおく．
$2k = (2, 2), \, h = (\theta - 1, M - 1)$より，$\lambda = \min \bigl\{ \theta/2, M/2 \bigr\}$．

$\theta < M$のとき．
$\lambda = \theta/2, \, m = 1$より
\begin{align}
\frac{1}{(m - 1)! 2^m \prod_{j=1}^m k_j}
& =
\frac{1}{2}, \nonumber \\
\mu_2
& =
M - \theta - 1 \nonumber \\
\delta \bigl( t - K(x, y) \bigr) x^{\theta - 1} r^{M - 1}
& \simeq
\frac{1}{2} t^{\theta/2 - 1} \delta(x) r^{M - \theta - 1} \nonumber
\end{align}

$\theta > M$のとき．
$\lambda = M/2, \, m = 1$より
\begin{align}
\frac{1}{(m - 1)! 2^m \prod_{j=1}^m k_j}
& =
\frac{1}{\theta}, \nonumber \\
\mu_2
& =
\theta - M - 1 \nonumber \\
\delta \bigl( t - K(x, y) \bigr) x^{\theta - 1} r^{M - 1}
& \simeq
\frac{1}{2} t^{M/2 - 1} x^{\theta - M - 1} \delta(r) \nonumber
\end{align}

\end{document}
