\documentclass[11pt,a4paper]{jsarticle}

\usepackage{amsmath,amssymb}

\newcommand{\E}{\mathrm{E}}

\begin{document}

\begin{align}
\mathcal{G}_n (\alpha)
& =
\E_X \Bigl[ \log \E_w \bigl[ p (X | w)^{\alpha} \bigr] \Bigr]. \nonumber
\end{align}

\begin{align}
l_k (A)
& =
\frac{\E_w \bigl[ (\frac{\partial}{\partial \alpha})^k p (A | w)^{\alpha} \bigr]}{\E_w \bigl[ p (A | w)^{\alpha} \bigr]} \nonumber \\
& =
\frac{\E_w \bigl[ \{ \log p (A | w) \}^k p (A | w)^{\alpha} \bigr]}{\E_w \bigl[ p (A | w)^{\alpha} \bigr]}. \nonumber
\end{align}

\begin{align}
\frac{\partial}{\partial \alpha}l_k (A)
& =
l_{k+1} (A) - l_k (A) l_1 (A). \nonumber
\end{align}

\begin{align}
\mathcal{G}_n^{(1)} (\alpha)
& =
\E_X \bigl[ l_1 \bigr]. \nonumber
\end{align}

\begin{align}
\mathcal{G}_n^{(2)} (\alpha)
& =
\E_X \bigl[ l^{\prime}_1 \bigr] = \E_X \bigl[ l_2 - l_1^2 \bigr]. \nonumber
\end{align}

\begin{align}
\mathcal{G}_n^{(3)} (\alpha)
& =
\E_X \bigl[ l^{\prime}_2 - 2 l_1 l^{\prime}_1 \bigr] \nonumber \\
& =
\E_X \bigl[ l_3 - 3 l_2 l_1 + 2 l_1^3 \bigr]. \nonumber
\end{align}

\begin{align}
\mathcal{G}_n^{(4)} (\alpha)
& =
\E_X \bigl[ l^{\prime}_3 - 3 l^{\prime}_2 l_1 - 3 l_2 l^{\prime}_1 + 6 l_1^2 l^{\prime}_1 \bigr] \nonumber \\
& =
\E_X \bigl[ l_4 - 4 l_3 l_1 - 3 l_2^2 + 12 l_2 l_1^2 - 6 l_1^4 \bigr]. \nonumber
\end{align}

\begin{align}
\mathcal{L}_k (A)
& =
\frac{\E_w \bigl[ (\frac{\partial}{\partial \alpha})^k e^{- \alpha f (A, w)} \bigr]}{\E_w \bigl[ e^{- \alpha f (A, w)} \bigr]} \nonumber \\
& =
\frac{\E_w \bigl[ \{ -f (A, w) \}^k e^{- \alpha f (A, w)} \bigr]}{\E_w \bigl[ e^{- \alpha f (A, w)} \bigr]}. \nonumber
\end{align}

\begin{align}
\frac{\partial}{\partial \alpha} \mathcal{L}_k (A)
& =
\mathcal{L}_{k+1} (A) - \mathcal{L}_k (A) \mathcal{L}_1 (A). \nonumber
\end{align}

\begin{align}
\mathcal{G}_n (\alpha)
& =
- \alpha L (w_0) + \E_X \Bigl[ \log \E_w \bigl[ e^{- \alpha f (X, w)} \bigr] \Bigr]. \nonumber
\end{align}

\begin{align}
\E_w^{(\alpha)} \bigl[ g (A, w) \bigr]
& =
\frac{\E_w \bigl[ g (A, w) e^{- \alpha f (A, w)} \bigr]}{\E_w \bigl[ e^{- \alpha f (A, w)} \bigr]}, \nonumber \\
\mathcal{L}_k (A)
& =
\E_w^{(\alpha)} \bigl[ \{ -f (A, w) \}^k \bigr]. \nonumber
\end{align}

\begin{align}
\overline{\mathcal{L}}_k (A)
& =
\E_w^{(\alpha)} \bigl[ | f (A, w) |^k \bigr]. \nonumber
\end{align}

$j \leq k$に対して
\begin{align}
| \mathcal{L}_j (A) |
& \leq
\overline{\mathcal{L}}_j (A) \leq \overline{\mathcal{L}}_k (A)^{j/k}. \nonumber
\end{align}

\begin{align}
\bigl| \mathcal{G}_n^{(2)} (\alpha) \bigr|
& \leq
\E_X \bigl[ |\mathcal{L}_2| + |\mathcal{L}_1|^2 \bigr] \nonumber \\
& \leq
\E_X \bigl[ \overline{\mathcal{L}}_2 + \overline{\mathcal{L}}_2 \bigr] \nonumber \\
& =
2 \E_X \bigl[ \overline{\mathcal{L}}_2 \bigr]. \nonumber
\end{align}

\begin{align}
\bigl| \mathcal{G}_n^{(3)} (\alpha) \bigr|
& \leq
\E_X \bigl[ |\mathcal{L}_3| + 3 |\mathcal{L}_2| |\mathcal{L}_1| + 2 |\mathcal{L}_1|^3 \bigr] \nonumber \\
& \leq
\E_X \bigl[ \overline{\mathcal{L}}_3 + 3 \overline{\mathcal{L}}_3 + 2 \overline{\mathcal{L}}_3 \bigr] \nonumber \\
& =
6 \E_X \bigl[ \overline{\mathcal{L}}_3 \bigr]. \nonumber
\end{align}

\begin{align}
\bigl| \mathcal{G}_n^{(4)} (\alpha) \bigr|
& \leq
\E_X \bigl[ |\mathcal{L}_4| + 4 |\mathcal{L}_3| |\mathcal{L}_1| + 3 |\mathcal{L}_2|^2 + 12 |\mathcal{L}_2| |\mathcal{L}_1|^2 + 6 |\mathcal{L}_1|^4 \bigr] \nonumber \\
& \leq
\E_X \bigl[ \overline{\mathcal{L}}_4 + 4 \overline{\mathcal{L}}_4 + 3 \overline{\mathcal{L}}_4 + 12 \overline{\mathcal{L}}_4 + 6 \overline{\mathcal{L}}_4 \bigr] \nonumber \\
& =
26 \E_X \bigl[ \overline{\mathcal{L}}_4	 \bigr]. \nonumber
\end{align}

\begin{align}
\E \bigl[ \mathcal{G}_{n-1} (\beta) \bigr]
& =
\E \biggl[ \E_X \Bigl[ \log \E_w \bigl[ p (X | w)^{\beta} \bigr] \Bigr] \biggr] \nonumber \\
& =
\E \biggl[ \int
\log \Bigl( \int p (x | w)^{\beta} \frac{1}{Z_{n-1} (\beta)} \prod_{i=1}^{n-1} p (X_i | w)^{\beta} \varphi (w) d w
\Bigr) q(x) \, d x \biggr] \nonumber \\
& =
\E \biggl[ \int
\log \Bigl( \int \frac{1}{Z_{n-1} (\beta)} \prod_{i=1}^n p (X_i | w)^{\beta} \varphi (w) d w
\Bigr) q(x) \, d x \biggr] \nonumber \\
& =
\E \Bigl[ \int \log \frac{Z_n (\beta)}{Z_{n-1} (\beta)} q(x) \, d x \Bigr] \nonumber \\
& =
\E \Bigl[ \log \frac{Z_n (\beta)}{Z_{n-1} (\beta)} \Bigr] \nonumber \\
& =
- \E \Bigl[ \log \frac{Z_{n-1} (\beta)}{Z_n (\beta)} \Bigr] \nonumber \\
& =
- \E \biggl[
\log \Bigl(
\int_W p (X_n | w)^{-\beta} \frac{1}{Z_n (\beta)} \prod_{i=1}^n p (X_i | w)^{\beta} \varphi (w) d w
\Bigr) \biggr] \nonumber \\
& =
- \E \Bigl[ \log \E_w \bigl[ p (X_n | w)^{-\beta} \bigr] \Bigr] \nonumber \\
& =
- \E \Bigl[ \frac{1}{n} \sum_{i=1}^n \log \E_w \bigl[ p (X_i | w)^{-\beta} \bigr] \Bigr] \nonumber \\
& =
- \E \bigl[ \mathcal{T}_n (-\beta) \bigr]. \nonumber
\end{align}

\end{document}
